Add proof that reset/trans projections of aig are Comb

Valaig/Aig/Projections.lean
@@ -1,7 +1,7 @@
 module
 
 import all Valaig.Aig.Basic
-public import Valaig.Aig.WellFormed
+public import Valaig.Aig.Semantics
 public import Valaig.Aig.Iter
 
 /-
@@ -11,8 +11,9 @@ These may go in the future, replaced by better methods for going straight to SAT
 
 public section
 namespace Valaig.Aig
+variable {aig : Aig} {wf : aig.WellFormed}
 
-def resetAig (aig : Aig) (wf : aig.WellFormed) : Aig :=
+private def projectComb (aig : Aig) (reset : Bool) (wf : aig.WellFormed) : Aig × (Lit.In aig -> Lit) :=
   go aig.iter .empty (.emptyWithCapacity aig.size)
 where
   go iter (state : Aig) (map : Array Lit)
@@ -20,45 +21,52 @@ where
     (valid : ∀ {lit} (_ : lit ∈ map), lit.validIn state := by grind) :=
     match h : iter.step.val with
     | .skip it => go iter state map
-    | .done => state
+    | .done =>
+      ⟨state, fun lit => lit.val.mapTo <| map[lit.val.var.idx]'(by grind [Var.validIn_eq_lt_size])⟩
     | .yield it' var =>
       let mapLit (lit : Lit) (h : lit.var < var := by grind) : Lit :=
         lit.mapTo map[lit.var.idx]
 
       let res : Aig × Lit := 
-        match h : aig[var] with
-        | .false => (state, .false)
-        | .input _ =>
+        match _ : reset, _ : aig[var] with
+        | _, .false => (state, .false)
+        | _, .input _ | false, .latch _ =>
           let (eq:=_) (state, idx) := state.addInput
           (state, idx.getLit state)
-        | .latch idx => (state, mapLit <| idx.getReset aig)
-        | .and rhs0 rhs1 => state.addAnd (mapLit rhs0) (mapLit rhs1)
+        | true, .latch idx => (state, mapLit <| idx.getReset aig)
+        | _, .and rhs0 rhs1 => state.addAnd (mapLit rhs0) (mapLit rhs1)
 
       go it' res.fst (map.push res.snd) (by simp; grind) (by simp [res]; grind)
   termination_by iter.length
   decreasing_by all_goals grind
 
-def transAig (aig : Aig) (wf : aig.WellFormed) : Aig :=
-  go aig.iter .empty (.emptyWithCapacity aig.size)
-where
-  go iter (state : Aig) (map : Array Lit)
-    (size : iter.var.idx = map.size := by grind)
-    (valid : ∀ {lit} (_ : lit ∈ map), lit.validIn state := by grind) :=
-    match h : iter.step.val with
-    | .skip it => go iter state map
-    | .done => state
-    | .yield it' var =>
-      let mapLit (lit : Lit) (h : lit.var < var := by grind) : Lit :=
-        lit.mapTo map[lit.var.idx]
+private theorem projectComb.Comb_go {reset iter size} (comb : state.Comb) :
+    (go aig reset wf iter state map size valid).fst.Comb := by
+  fun_induction go
+  · grind only
+  · grind only
+  next res ih =>
+    apply ih
+    subst res
+    grind
 
-      let res : Aig × Lit := 
-        match h : aig[var] with
-        | .false => (state, .false)
-        | .input _ | .latch _ =>
-          let (eq:=_) (state, idx) := state.addInput
-          (state, idx.getLit state)
-        | .and rhs0 rhs1 => state.addAnd (mapLit rhs0) (mapLit rhs1)
+@[local simp]
+private theorem Comb_projectComb :
+    (aig.projectComb reset wf).fst.Comb :=
+  projectComb.Comb_go (by simp)
 
-      go it' res.fst (map.push res.snd) (by simp; grind) (by simp [res]; grind)
-  termination_by iter.length
-  decreasing_by all_goals grind
+@[inline]
+def resetAig (aig : Aig) (wf : aig.WellFormed := by grind) : Aig × (Lit.In aig -> Lit) :=
+  projectComb aig true wf
+
+theorem Comb_resetAig :
+    (aig.resetAig wf).fst.Comb :=
+  Comb_projectComb
+
+@[inline]
+def transAig (aig : Aig) (wf : aig.WellFormed := by grind) : Aig × (Lit.In aig -> Lit) :=
+  projectComb aig false wf
+
+theorem Comb_transAig :
+    (aig.transAig wf).fst.Comb :=
+  Comb_projectComb
